Code/Reg_Exp_Prop.v
@@ -4,8 +4,9 @@ Require Import Reg_Exp.
 Lemma Reg_plus {A:Type} (e1 : @Reg_Exp A) :
     Plus e1 e1  = e1.
 Proof.
+induction e1.
 destruct Plus.
--
+reflexivity.
 
 
 
